iris/UShPipesStage.v
@@ -61,8 +61,30 @@ Require Import UShPipeAssembly.   (* [ksh_w1_of_step], [alt_execfail_app] *)
 Require Import UkConsOut.   (* [cons_short] *)
 Require Import UkPipesIface UkPipesEntries.
 Require Import PipesFire UShPipesDefs.
+Require ExecWords UkShDiagAt FileDisc.
 Require User.ShSyms.
 Local Open Scope Z_scope.
+
+(* sh's [exec cat failed], around the command's name *)
+Lemma catf_execfail_bytes : UkShDiagAt.ush_execfail_bytes alt_execR FileDisc.fd_w_cat.
+Proof using .
+  rewrite /UkShDiagAt.ush_execfail_bytes. split_and!.
+  - vm_compute. lia.
+  - intros j Hj.
+    assert (Hl : (j < length alt_execR)%nat) by (vm_compute in Hj |- *; lia).
+    exact (list_lookup_lookup_total_lt alt_execR j Hl).
+  - intros j Hj.
+    apply (UkShDiag.ush_bytes_of_forallb (UkShDiag.shd_lit 0x12a8)
+             (fun i : nat => alt_execR !!! i) 0%nat 5%nat);
+      [vm_compute; reflexivity | lia].
+  - intros j Hj.
+    assert (Hj3 : (j < 3)%nat) by (vm_compute in Hj; lia).
+    destruct j as [| [| [| j]]]; try lia; vm_compute; reflexivity.
+  - intros j Hj.
+    apply (UkShDiag.ush_bytes_of_forallb (UkShDiag.shd_lit 0x12a8)
+             (fun i : nat => alt_execR !!! (i + 1)%nat) 7%nat 8%nat);
+      [vm_compute; reflexivity | lia].
+Qed.
 
 Section UShPipesStage.
   (* [UShPipeLaw]'s binder list, and C6's two classes *)
@@ -89,6 +111,8 @@ Section UShPipesStage.
   Context (v : era_pins) (I : list (bv 8)).
   Context (Hadmit : pns_adm fc adm I) (Hplok : pl_ok (lineN fc adm I)).
   Context (L : list (bv 8)) (HL31 : pns_short L).
+  (* THE PRODUCER at the head of the line *)
+  Context (pr : producer).
   Context (γc γm : wid -> gname).
   Context (P : nat -> pnames) (gF gG : nat -> gname).
 
@@ -101,10 +125,10 @@ Section UShPipesStage.
   Local Notation PWN := (pwc_blkN g fc adm v I).
   Local Notation WITN := (pwitN fc adm I).
   Local Notation TOKN := (tokN fc (lineN fc adm I)).
-  Local Notation pdepR := (pdep fc adm I L P gF gG).
+  Local Notation pdepR := (pdep fc adm I L pr P gF gG).
   Local Notation FAM := (blkN_inv wsN RUNN PWN termw TOKN pdepR pnsN (S gen_id) γc γm).
   Local Notation pkitR w s := (pns_kit fc adm I termw TOKN pdepR w s).
-  Local Notation QcR k := (QcK g fc adm v I L γc γm P k).
+  Local Notation QcR k := (QcK g fc adm v I L pr γc γm P k).
   Local Notation a0_idx := (mword_of_int 10 : mword 5).
 
   (* ================================================================= *)
@@ -149,13 +173,13 @@ Section UShPipesStage.
       destruct p as [| p'].
       + iDestruct "HF" as "(Hc & Hm & Hd)".
         iApply (pipesN_fire g fc adm LW Hcons Hfc v I Hadmit Hplok pnsN (↑pipeN) (S gen_id)
-                  γc γm termw TOKN pdepR (pdep_timeless fc adm I L P gF gG) w s b EX Φ
+                  γc γm termw TOKN pdepR (pdep_timeless fc adm I L pr P gF gG) w s b EX Φ
                   pnsN_uart pnsN_pipeN Hw (Hdg 0%nat b Hp Hb) Hok
                   with "Hex Hinv Hc Hm Hd").
         iIntros "Hc Hm #HT". iApply "HΦ". iFrame "HR Hc Hm HT".
       + iDestruct "HF" as "(Hc & Hm & #HT)".
         iApply (pipesN_cstep g fc adm LW Hcons Hfc v I Hadmit Hplok pnsN (S gen_id)
-                  γc γm termw TOKN pdepR (pdep_timeless fc adm I L P gF gG) w s (S p') b Φ
+                  γc γm termw TOKN pdepR (pdep_timeless fc adm I L pr P gF gG) w s (S p') b Φ
                   pnsN_uart Hw ltac:(lia) (Hdg (S p') b Hp Hb) (Hst (S p') ltac:(lia))
                   with "Hinv Hc Hm").
         iIntros "Hc Hm _". iApply "HΦ". iFrame "HR Hc Hm HT".
@@ -180,8 +204,8 @@ Section UShPipesStage.
 
   (* THE ROUND'S FIRING PREMISE: every commit a process of the round
      makes is admitted by the model, or refuted by a committed deposit *)
-  Hypothesis Hfire : forall w s, w ∈ wsN -> fire_src L w s ->
-    fire_okN wsN RUNN WITN termw TOKN w s (EXf nc L w s).
+  Hypothesis Hfire : forall w s, w ∈ wsN -> fire_src fc pr L w s ->
+    fire_okN wsN RUNN WITN termw TOKN w s (EXf fc pr nc L w s).
 
   Lemma dg_execL_len : length dg_execL = 17%nat.
   Proof using . vm_compute. reflexivity. Qed.
@@ -202,7 +226,7 @@ Section UShPipesStage.
   Lemma stage_echo (ws : list (list (bv 8))) (s0 : Z) (gs : nat -> bv 8)
       (N' : uk_names Σ) (h' : CpuId) (m' : regfile) (γp : pipe_names) (q szv : Z)
       (ld : list fdstate) (av : nat) :
-    line_ok ws -> echo_argv_bytes ws gs -> L = wl_line (drop 1 ws) -> L <> [] ->
+    pr = PrEcho ws -> line_ok ws -> echo_argv_bytes ws gs -> L = wl_line (drop 1 ws) ->
     (0 < nc)%nat ->
     ukn_pay N' = (fun _ : Z => QcR 0) ->
     m' !!! Regidx a0_idx = (mword_of_int q : mword 64) ->
@@ -218,7 +242,8 @@ Section UShPipesStage.
       (2 + (UkShDiag.ush_Dg + av)) -∗
     mWP (Loop : expr riscv_lang).
   Proof using HL31 Hadmit Hcons Heq Hfc Hfire Hkill Hplok pnsRegG0.
-    intros Hok Hbytes HLw HLne Hn Hpeq Ha0 Hfd1 Hfd2 Hav.
+    intros Hpr Hok Hbytes HLw Hn Hpeq Ha0 Hfd1 Hfd2 Hav.
+    assert (Hdg0 : dg_execL = dg_st pr 0) by (rewrite Hpr; reflexivity).
     iIntros "#Hinv #Hslot #Hcode #Hjt #Hcmd Hsz Hstd Hcwd Hch Hraw Hrun".
     pose proof (ukn_const_of_eq N' _ Hpeq (fun x y => eq_refl)) as Hc.
     iDestruct "Hraw" as "(#Hpi & Hw & #Hlb & HsL & Hcw & Hmw & HG)".
@@ -238,7 +263,14 @@ Section UShPipesStage.
       - iIntros "!> (Hw & HsL & Hcw & Hmw)". rewrite /pns_echo_lend.
         iFrame "Hpi Hw Hlb". rewrite /pns_xkQ.
         iIntros "[#HT | [Hf _]]"; [by iLeft |].
-        cbn [pns_final snd]. rewrite /pns_lexit.
+        cbn [pns_final snd].
+        iDestruct "Hf" as "[Hf | Hw0]"; last first.
+        { (* the write end untouched: [WrNone] *)
+          iRight. iLeft. iFrame "HsL". rewrite /lrep. iExists None.
+          cbn [pns_wfin]. iFrame "Hcw Hmw". iRight. iExists WrNone.
+          cbn [wr_final]. rewrite /wtok.
+          iSplitL "Hw0"; [iExact "Hw0" | iPureIntro; intros D HD; discriminate HD]. }
+        rewrite /pns_lexit.
         iDestruct "Hf" as "[Hf | [Hf | #Hta]]"; last first.
         { iLeft. rewrite Hkill. iExact "Hta". }
         + iDestruct "Hf" as (c) "(%HcL & [Hw' #Hlb'] & #Hro)".
@@ -253,7 +285,7 @@ Section UShPipesStage.
           iSplitL; [| iPureIntro; intros D HD; by injection HD as <-].
           iFrame "Hlb'". by iLeft.
       - iApply (pse_echo_image_entry (PS := uprogSG_free) g fc adm LW Hcons Hkill rn Heq Hfc
-                  v I Hadmit Hplok L HL31 termw TOKN pdepR (pdep_timeless fc adm I L P gF gG)
+                  v I Hadmit Hplok L HL31 termw TOKN pdepR (pdep_timeless fc adm I L pr P gF gG)
                   γc γm ws M s1 t1 g1 sts FsImg.ROOTINO cs pidv rb (fun _ : Z => QcR 0)
                   (P 0) γp (fun _ _ => eq_refl) Hok Hi1 Hb1 Hl1 Hr1 HLw
                   with "Hnp []").
@@ -264,20 +296,20 @@ Section UShPipesStage.
       as "#Hxl".
     { rewrite /UkShDiag.ush_execfail_law.
       iApply (exf_writer (WLeft 0) dg_execL EchoDisc.alt_execfail 17%nat
-                (EXf nc L (WLeft 0) dg_execL) Cr (side_L (P 0)) Cd Hw0 ltac:(lia)
+                (EXf fc pr nc L (WLeft 0) dg_execL) Cr (side_L (P 0)) Cd Hw0 ltac:(lia)
                 ltac:(intros p b Hp Hb; rewrite alt_execfail_app in Hb;
                       exact (dg_app_lookup dg_execL u_prompt p b
                                ltac:(rewrite dg_execL_len; lia) Hb))
-                (Hfire (WLeft 0) dg_execL Hw0 (or_introl eq_refl))
+                (Hfire (WLeft 0) dg_execL Hw0 (or_introl (or_introl Hdg0)))
                 ltac:(intros c Hcx; apply (cstep_okN_tok fc adm I Hadmit (WLeft 0) dg_execL c);
                       [lia | rewrite dg_execL_len; lia | intros k Hk; discriminate Hk])
                 with "Hinv [] [] []").
-      - iApply (pexcl_left fc adm I L P gF gG 0 dg_execL Hn (dg_st_ne 0) HLne).
+      - iApply (pexcl_left fc adm I L pr P gF gG 0 dg_execL Hn ltac:(vm_compute; discriminate)).
         rewrite /pinv. iExists γp. cbn [prevP flow_U]. iExact "Hpi".
       - iIntros "!> (Hw & HsL & Hcw & Hmw)". iFrame "HsL Hcw Hmw".
-        rewrite (pdep_unfold fc adm I L P gF gG (WLeft 0) dg_execL (dg_st_ne 0)
-                   (or_introl eq_refl)) /pdep_ne.
-        rewrite bool_decide_true; [| reflexivity].
+        rewrite (pdep_unfold fc adm I L pr P gF gG (WLeft 0) dg_execL
+                   ltac:(vm_compute; discriminate) (or_introl (or_introl Hdg0))) /pdep_ne.
+        rewrite bool_decide_true; [| left; exact Hdg0].
         iFrame "Hw HGs". rewrite /shotsF. done.
       - iIntros "!> HsL Hcw Hmw _". rewrite /Cd. iFrame "HsL".
         cbn [pns_wfin]. rewrite dg_execL_len. iFrame "Hcw Hmw". }
@@ -289,9 +321,152 @@ Section UShPipesStage.
               N' Hc h' m' q szv s0 gs ld (av - 6)%nat Hok Hpeq Ha0 Hbytes Hfd1 Hfd2
               with "Hcode Hsup Hxl [] Hjt Hcmd Hsz Hstd Hcwd [Hch] [Hw HsL Hcw Hmw] Hrun").
     - iIntros "!> [HsL Hf]". iRight. iLeft. iFrame "HsL". rewrite /lrep.
-      iExists (Some dg_execL). iFrame "Hf". by iLeft.
+      iExists (Some dg_execL). iFrame "Hf". iLeft. iPureIntro.
+      exists dg_execL. split; [reflexivity | left; exact Hdg0].
     - iApply (UserChildren.uch_any_of with "Hch").
     - rewrite /Cr. iFrame.
+  Qed.
+
+  (* ================================================================= *)
+  (*  2b. THE PRODUCER'S STAGE LAW, and [cat f] AT THE HEAD              *)
+  (* ================================================================= *)
+
+  (* WHAT NODE 0'S LEFT CHILD DOES, whatever the producer: sh's exec arm
+     at the stage's command [args0], on node 0's lend [echo_raw], paying
+     node 0's side-tagged report.  Echo's is [stage_echo]
+     ([stage_echo_law]); [cat f]'s is [stage_catf] at the entry C9d'
+     builds ([stage_catf_law]). *)
+  Definition prod_stage_law (args0 : list uarg) : iProp Σ :=
+    (□ (∀ (N' : uk_names Σ) (h' : CpuId) (m' : regfile) (γp : pipe_names) (q szv : Z)
+          (ld : list fdstate) (av : nat),
+          ⌜ukn_pay N' = (fun _ : Z => QcR 0)⌝ -∗
+          ⌜m' !!! Regidx a0_idx = (mword_of_int q : mword 64)⌝ -∗
+          ⌜UShEchoPipePay.ush_fd1pipe γp ld⌝ -∗ ⌜UkSh.ush_fd2p ld⌝ -∗ ⌜(6 <= av)%nat⌝ -∗
+          shk_code (ukn_t N') -∗ ush_jtab (ukn_t N') -∗
+          ush_cmd (ukn_d N') q (UExec args0) -∗
+          usz (ukn_s N') szv -∗ UserFd.ustd (ukn_fd N') ld -∗
+          UserCwd.ucwd (ukn_cwd N') FsImg.ROOTINO -∗
+          UserChildren.uch (ukn_ch N') (∅ : gset gname) -∗
+          echo_raw γp -∗
+          urun (SG := uexecSG_xv6) (PS := uprogSG_free) N' h' m' (mword_of_int ShSyms.runcmd)
+            (2 + (UkShDiag.ush_Dg + av)) -∗
+          mWP (Loop : expr riscv_lang)))%I.
+
+  Global Instance prod_stage_law_persistent args0 : Persistent (prod_stage_law args0) | 0.
+  Proof using . rewrite /prod_stage_law. apply bi.intuitionistically_persistent. Qed.
+
+  Lemma stage_echo_law (ws : list (list (bv 8))) (s0 : Z) (gs : nat -> bv 8) :
+    pr = PrEcho ws -> line_ok ws -> echo_argv_bytes ws gs -> L = wl_line (drop 1 ws) ->
+    (0 < nc)%nat ->
+    FAM -∗ UShEcho.sh_echo_slot T -∗
+    prod_stage_law (UkShMain.ush_args s0 gs (echo_toks ws)).
+  Proof using HL31 Hadmit Hcons Heq Hfc Hfire Hkill Hplok pnsRegG0.
+    intros Hpr Hok Hbytes HLw Hn. iIntros "#Hfam #Hes". rewrite /prod_stage_law.
+    iIntros "!>" (N' h' m' γp q szv ld av) "%Hpeq %Ha0 %Hfd1 %Hfd2 %Hav #Hck #Hjt #Hcmd".
+    iIntros "Hsz Hstd Hcwd Hch Hraw Hrun".
+    iApply (stage_echo ws s0 gs N' h' m' γp q szv ld av Hpr Hok Hbytes HLw Hn Hpeq Ha0
+              Hfd1 Hfd2 Hav with "Hfam Hes Hck Hjt Hcmd Hsz Hstd Hcwd Hch Hraw Hrun").
+  Qed.
+
+  (* what the head stage holds at its exec: the first pipe's write permit,
+     its side token and the stage's family writer ([stage_echo]'s [Cr]) *)
+  Definition prod_cr : iProp Σ :=
+    (wcur (P 0) 0 ∗ side_L (P 0)
+     ∗ wcurN γc (WLeft 0) (1/2) 0 ∗ wmodeN γm (WLeft 0) (1/2) None)%I.
+
+
+  (* [cat f] AT THE HEAD (union.md S6, C9c').  The exec arm at the words
+     [cat f]: the EXEC SUCCEEDS arm is the ENTRY, a premise here -- C9d'
+     builds it at the merged registry (the [cat f] image, fd 1 the first
+     pipe's write end at [DOutH [L; []]], fd 2 the stage's family writer
+     at [[]; cat: cannot open f; cat: write error]); the EXEC FAILS arm is
+     the stage's family writer at [exec cat failed], depositing its
+     untouched write permit, as echo's does. *)
+  Lemma stage_catf (f : list (bv 8)) (s0 : Z) (gs : nat -> bv 8)
+      (N' : uk_names Σ) (h' : CpuId) (m' : regfile) (γp : pipe_names) (q szv : Z)
+      (ld : list fdstate) (av : nat) :
+    pr = PrCatF f -> ExecWords.exec_ok (FileDisc.prod_words (PrCatF f)) ->
+    echo_argv_bytes (FileDisc.prod_words (PrCatF f)) gs ->
+    (0 < nc)%nat ->
+    ukn_pay N' = (fun _ : Z => QcR 0) ->
+    m' !!! Regidx a0_idx = (mword_of_int q : mword 64) ->
+    UShEchoPipePay.ush_fd1pipe γp ld -> UkSh.ush_fd2p ld -> (6 <= av)%nat ->
+    FAM -∗
+    (* THE ENTRY: exec'ing [cat f] on the stage's lend pays node 0's report *)
+    UkShEcho.sh_exec_sup_echo_at (SG := uexecSG_xv6)
+      (UShEchoPipePay.ush_fd1pipe γp) (FileDisc.prod_words (PrCatF f))
+      (fun _ : Z => QcR 0) prod_cr -∗
+    shk_code (ukn_t N') -∗ ush_jtab (ukn_t N') -∗
+    ush_cmd (ukn_d N') q (echo_cmd (FileDisc.prod_words (PrCatF f)) s0 gs) -∗
+    usz (ukn_s N') szv -∗ UserFd.ustd (ukn_fd N') ld -∗
+    UserCwd.ucwd (ukn_cwd N') FsImg.ROOTINO -∗
+    UserChildren.uch (ukn_ch N') (∅ : gset gname) -∗
+    echo_raw γp -∗
+    urun (SG := uexecSG_xv6) (PS := uprogSG_free) N' h' m' (mword_of_int ShSyms.runcmd)
+      (2 + (UkShDiag.ush_Dg + av)) -∗
+    mWP (Loop : expr riscv_lang).
+  Proof using Hadmit Hcons Hfc Hfire Hplok.
+    intros Hpr Hok Hbytes Hn Hpeq Ha0 Hfd1 Hfd2 Hav.
+    assert (Hdg0 : dg_execR = dg_st pr 0) by (rewrite Hpr; reflexivity).
+    iIntros "#Hinv #Hsup #Hcode #Hjt #Hcmd Hsz Hstd Hcwd Hch Hraw Hrun".
+    pose proof (ukn_const_of_eq N' _ Hpeq (fun x y => eq_refl)) as Hc.
+    iDestruct "Hraw" as "(#Hpi & Hw & #Hlb & HsL & Hcw & Hmw & HG)".
+    iApply stg_fupd_mwp. iMod (os_shoot with "HG") as "#HGs". iModIntro.
+    assert (Hw0 : WLeft 0 ∈ wsN) by (apply wids_elem; exact Hn).
+    set (Cd := (side_L (P 0) ∗ pns_wfin γc γm (WLeft 0) (Some dg_execR))%I).
+    (* ---- THE EXEC-FAILED LAW: the stage's family writer ---- *)
+    iAssert (UkShDiag.ush_execfail_law_at (SG := uexecSG_xv6) (PS := uprogSG_free)
+               alt_execR 16%nat prod_cr Cd)%I as "#Hxl".
+    { iApply (exf_writer (WLeft 0) dg_execR alt_execR 16%nat
+                (EXf fc pr nc L (WLeft 0) dg_execR) prod_cr (side_L (P 0)) Cd Hw0 ltac:(lia)
+                ltac:(intros j b Hj Hb; exact (dg_app_lookup dg_execR u_prompt j b
+                               ltac:(rewrite dg_execR_len; lia) Hb))
+                (Hfire (WLeft 0) dg_execR Hw0 (or_introl (or_introl Hdg0)))
+                ltac:(intros c Hcx; apply (cstep_okN_tok fc adm I Hadmit (WLeft 0) dg_execR c);
+                      [lia | rewrite dg_execR_len; lia | intros k Hk; discriminate Hk])
+                with "Hinv [] [] []").
+      - iApply (pexcl_left fc adm I L pr P gF gG 0 dg_execR Hn ltac:(vm_compute; discriminate)).
+        rewrite /pinv. iExists γp. cbn [prevP flow_U]. iExact "Hpi".
+      - iIntros "!> (Hw & HsL & Hcw & Hmw)". iFrame "HsL Hcw Hmw".
+        rewrite (pdep_unfold fc adm I L pr P gF gG (WLeft 0) dg_execR
+                   ltac:(vm_compute; discriminate) (or_introl (or_introl Hdg0))) /pdep_ne.
+        rewrite bool_decide_true; [| left; exact Hdg0].
+        iFrame "Hw HGs". rewrite /shotsF. done.
+      - iIntros "!> HsL Hcw Hmw _". rewrite /Cd. iFrame "HsL".
+        cbn [pns_wfin]. rewrite dg_execR_len. iFrame "Hcw Hmw". }
+    (* ---- ...AND THE ARM, at any exec'able word list ---- *)
+    replace (2 + (UkShDiag.ush_Dg + av))%nat
+      with (6 + (2 + (UkShDiag.ush_Dg + (av - 6))))%nat by lia.
+    iApply (UkShEcho.wp_kshr_exec_x_at_holds (SG := uexecSG_xv6) (PS := uprogSG_free)
+              (UShEchoPipePay.ush_fd1pipe γp) (FileDisc.prod_words (PrCatF f)) alt_execR
+              (fun _ : Z => QcR 0) prod_cr Cd
+              N' Hc h' m' q szv s0 gs ld (av - 6)%nat Hok catf_execfail_bytes Hpeq Ha0
+              Hbytes Hfd1 Hfd2
+              with "Hcode Hsup Hxl [] Hjt Hcmd Hsz Hstd Hcwd [Hch] [Hw HsL Hcw Hmw] Hrun").
+    - iIntros "!> [HsL Hf]". iRight. iLeft. iFrame "HsL". rewrite /lrep.
+      iExists (Some dg_execR). iFrame "Hf". iLeft. iPureIntro.
+      exists dg_execR. split; [reflexivity | left; exact Hdg0].
+    - iApply (UserChildren.uch_any_of with "Hch").
+    - rewrite /prod_cr. iFrame.
+  Qed.
+
+  (* ...AS THE PRODUCER'S STAGE LAW, at the entry *)
+  Lemma stage_catf_law (f : list (bv 8)) (s0 : Z) (gs : nat -> bv 8) :
+    pr = PrCatF f -> ExecWords.exec_ok (FileDisc.prod_words (PrCatF f)) ->
+    echo_argv_bytes (FileDisc.prod_words (PrCatF f)) gs -> (0 < nc)%nat ->
+    FAM -∗
+    □ (∀ γp : pipe_names,
+         UkShEcho.sh_exec_sup_echo_at (SG := uexecSG_xv6)
+           (UShEchoPipePay.ush_fd1pipe γp) (FileDisc.prod_words (PrCatF f))
+           (fun _ : Z => QcR 0) prod_cr) -∗
+    prod_stage_law (UkShMain.ush_args s0 gs (echo_toks (FileDisc.prod_words (PrCatF f)))).
+  Proof using Hadmit Hcons Hfc Hfire Hplok.
+    intros Hpr Hok Hbytes Hn. iIntros "#Hfam #Hsup". rewrite /prod_stage_law.
+    iIntros "!>" (N' h' m' γp q szv ld av) "%Hpeq %Ha0 %Hfd1 %Hfd2 %Hav #Hck #Hjt #Hcmd".
+    iIntros "Hsz Hstd Hcwd Hch Hraw Hrun".
+    iApply (stage_catf f s0 gs N' h' m' γp q szv ld av Hpr Hok Hbytes Hn Hpeq Ha0
+              Hfd1 Hfd2 Hav with "Hfam [] Hck Hjt Hcmd Hsz Hstd Hcwd Hch Hraw Hrun").
+    iApply "Hsup".
   Qed.
 
   #[local] Instance stg_kit_pers0 w s : Persistent (pkitR w s) | 0 :=
@@ -300,13 +475,14 @@ Section UShPipesStage.
   Lemma cons_short_A2 : cons_short [[]; cat_dg_write].
   Proof using . rewrite /cons_short. repeat constructor; vm_compute; reflexivity. Qed.
 
+  (* a halted cat's deposit: a middle cat, or the [cat f] producer *)
   Lemma pdep_left_write (k : nat) :
-    k <> 0%nat -> shotsF gF k -∗ osS (gG k) -∗ pdepR (WLeft k) cat_dg_write.
+    (k <> 0%nat \/ prod_halts fc pr) -> shotsF gF k -∗ osS (gG k) -∗ pdepR (WLeft k) cat_dg_write.
   Proof using .
     intros Hk. iIntros "#Hs #HG".
-    rewrite (pdep_unfold fc adm I L P gF gG (WLeft k) cat_dg_write
+    rewrite (pdep_unfold fc adm I L pr P gF gG (WLeft k) cat_dg_write
                ltac:(vm_compute; discriminate) (or_intror (conj Hk eq_refl))) /pdep_ne.
-    rewrite bool_decide_false; [| intros Hq; exact (dg_st_ne_write k (eq_sym Hq))].
+    rewrite bool_decide_false; [| intros Hq; exact (fail_src_ne_write pr k _ Hq eq_refl)].
     iFrame "Hs HG".
   Qed.
 
@@ -333,7 +509,7 @@ Section UShPipesStage.
   Lemma stage_mid (k' a b : nat) (s0 : Z) (gs : nat -> bv 8)
       (N' : uk_names Σ) (h' : CpuId) (m' : regfile) (gin γp : pipe_names) (q szv : Z)
       (ld : list fdstate) (av : nat) :
-    UkShCat.cat_argv_bytes a b gs -> L <> [] -> (S k' < nc)%nat ->
+    UkShCat.cat_argv_bytes a b gs -> (S k' < nc)%nat ->
     ukn_pay N' = (fun _ : Z => QcR (S k')) ->
     m' !!! Regidx a0_idx = (mword_of_int q : mword 64) ->
     mid_fd0 gin γp ld -> (6 <= av)%nat ->
@@ -348,7 +524,7 @@ Section UShPipesStage.
       (2 + (UkShDiag.ush_Dg + av)) -∗
     mWP (Loop : expr riscv_lang).
   Proof using HL31 Hadmit Hcons Heq Hfc Hfire Hkill Hplok pnsRegG0 uartGhostG0.
-    intros Hbytes HLne Hk Hpeq Ha0 Hfd Hav.
+    intros Hbytes Hk Hpeq Ha0 Hfd Hav.
     iIntros "#Hinv #Hslot #Hcode #Hjt #Hcmd Hsz Hstd Hcwd Hch Hraw Hrun".
     pose proof (ukn_const_of_eq N' _ Hpeq (fun x y => eq_refl)) as Hc.
     iDestruct "Hraw" as "(#Hpin & #Hpo & Hr & Hw & #Hlb & HsL & Hcw & Hmw & HG & #Hsk)".
@@ -359,11 +535,11 @@ Section UShPipesStage.
     { rewrite /pinv. iExists γp. cbn [prevP]. iExact "Hpo". }
     iAssert (pkitR (WLeft (S k')) cat_dg_write) as "#Hkw".
     { rewrite /pns_kit. iSplit.
-      - iExists (EXf nc L (WLeft (S k')) cat_dg_write). iSplitR.
+      - iExists (EXf fc pr nc L (WLeft (S k')) cat_dg_write). iSplitR.
         + iPureIntro. apply (Hfire (WLeft (S k')) cat_dg_write Hwk).
-          cbn [fire_src]. right. split; [lia | reflexivity].
-        + iApply (pexcl_left fc adm I L P gF gG (S k') cat_dg_write Hk
-                    ltac:(vm_compute; discriminate) HLne with "Hpk").
+          cbn [fire_src]. right. split; [left; lia | reflexivity].
+        + iApply (pexcl_left fc adm I L pr P gF gG (S k') cat_dg_write Hk
+                    ltac:(vm_compute; discriminate) with "Hpk").
       - iPureIntro. intros c [Hc0 Hcl].
         apply (cstep_okN_tok fc adm I Hadmit (WLeft (S k')) cat_dg_write c Hc0 Hcl).
         intros j Hj; discriminate Hj. }
@@ -395,7 +571,7 @@ Section UShPipesStage.
         iSplitR; [iExact "Hinv" |]. iFrame "Hcw Hmw".
         iSplitR.
         { rewrite /A2. iSplitR; [by iLeft |]. iSplitR; [| done]. iRight.
-          iFrame "Hkw". iApply (pdep_left_write (S k') ltac:(lia) with "Hsk HGs"). }
+          iFrame "Hkw". iApply (pdep_left_write (S k') ltac:(left; lia) with "Hsk HGs"). }
         rewrite /pns_xkQ. iIntros "[#HT | (Hf0 & Hf1 & _)]"; [by iLeft |].
         cbn [pns_final snd].
         iDestruct "Hf0" as (o) "[_ Ho]".
@@ -415,7 +591,7 @@ Section UShPipesStage.
           iExists RdGone. cbn [rd_final]. iSplit; [done |].
           iPureIntro. intros D HD. discriminate HD.
       + iApply (pse_mid_image_entry (PS := uprogSG_free) g fc adm LW Hcons Hkill rn Heq Hfc
-                  v I Hadmit Hplok L HL31 termw TOKN pdepR (pdep_timeless fc adm I L P gF gG)
+                  v I Hadmit Hplok L HL31 termw TOKN pdepR (pdep_timeless fc adm I L pr P gF gG)
                   γc γm a b M s1 t1 g1 sts FsImg.ROOTINO cs pidv (fun _ : Z => QcR (S k'))
                   (WLeft (S k')) A2 A2 (P k') gin (P (S k')) γp wb rb1 rb2
                   (fun _ _ => eq_refl) Ht1 Hs1 Hb1 Hi1 Hl1 Hr0 Hr1 Hr2
@@ -424,26 +600,27 @@ Section UShPipesStage.
         iApply UexecExecMint.udep_free.
     - (* ---- THE EXEC-FAILED LAW: the stage's family writer ---- *)
       iApply (exf_writer (WLeft (S k')) dg_execR alt_execR 16%nat
-                (EXf nc L (WLeft (S k')) dg_execR) Cr (side_L (P (S k'))) Cd Hwk ltac:(lia)
+                (EXf fc pr nc L (WLeft (S k')) dg_execR) Cr (side_L (P (S k'))) Cd Hwk ltac:(lia)
                 ltac:(intros p b' Hp Hb; exact (dg_app_lookup dg_execR u_prompt p b'
                                ltac:(rewrite dg_execR_len; lia) Hb))
-                (Hfire (WLeft (S k')) dg_execR Hwk (or_introl eq_refl))
+                (Hfire (WLeft (S k')) dg_execR Hwk (or_introl (or_introl eq_refl)))
                 ltac:(intros c Hcx;
                       apply (cstep_okN_tok fc adm I Hadmit (WLeft (S k')) dg_execR c);
                       [lia | rewrite dg_execR_len; lia | intros j Hj; discriminate Hj])
                 with "Hinv [] [] []").
-      + iApply (pexcl_left fc adm I L P gF gG (S k') dg_execR Hk (dg_st_ne (S k')) HLne
+      + iApply (pexcl_left fc adm I L pr P gF gG (S k') dg_execR Hk (dg_st_ne pr (S k'))
                   with "Hpk").
       + iIntros "!> (_ & Hw & HsL & Hcw & Hmw)". iFrame "HsL Hcw Hmw".
-        rewrite (pdep_unfold fc adm I L P gF gG (WLeft (S k')) dg_execR (dg_st_ne (S k'))
-                   (or_introl eq_refl))
+        rewrite (pdep_unfold fc adm I L pr P gF gG (WLeft (S k')) dg_execR (dg_st_ne pr (S k'))
+                   (or_introl (or_introl eq_refl)))
           /pdep_ne.
-        rewrite bool_decide_true; [| reflexivity].
+        rewrite bool_decide_true; [| by left].
         iFrame "Hw HGs Hsk".
       + iIntros "!> HsL Hcw Hmw _". rewrite /Cd. iFrame "HsL".
         cbn [pns_wfin]. rewrite dg_execR_len. iFrame "Hcw Hmw".
     - iIntros "!> [HsL Hf]". iRight. iLeft. iFrame "HsL". rewrite /lrep.
-      iExists (Some dg_execR). iFrame "Hf". by iLeft.
+      iExists (Some dg_execR). iFrame "Hf". iLeft. iPureIntro.
+      exists dg_execR. split; [reflexivity | by left].
     - iApply (UserChildren.uch_any_of with "Hch").
     - rewrite /Cr. iFrame.
   Qed.
@@ -473,7 +650,7 @@ Section UShPipesStage.
   Lemma stage_last (m a b : nat) (s0 : Z) (gs : nat -> bv 8)
       (N' : uk_names Σ) (h' : CpuId) (m' : regfile) (γp : pipe_names) (q szv : Z)
       (ld : list fdstate) (av : nat) :
-    UkShCat.cat_argv_bytes a b gs -> L <> [] -> nc = S m ->
+    UkShCat.cat_argv_bytes a b gs -> nc = S m ->
     ukn_pay N' = (fun _ : Z => QcR m) ->
     m' !!! Regidx a0_idx = (mword_of_int q : mword 64) ->
     last_fd0 γp ld -> (6 <= av)%nat ->
@@ -488,7 +665,7 @@ Section UShPipesStage.
       (2 + (UkShDiag.ush_Dg + av)) -∗
     mWP (Loop : expr riscv_lang).
   Proof using HL31 Hadmit Hcons Heq Hfc Hfire Hkill Hplok pnsRegG0 uartGhostG0.
-    intros Hbytes HLne Hm Hpeq Ha0 Hfd Hav.
+    intros Hbytes Hm Hpeq Ha0 Hfd Hav.
     iIntros "#Hinv #Hslot #Hcode #Hjt #Hcmd Hsz Hstd Hcwd Hch Hraw Hrun".
     pose proof (ukn_const_of_eq N' _ Hpeq (fun x y => eq_refl)) as Hc.
     iDestruct "Hraw" as "(#Hpo & #Hinvs & Hr & HsR & Hcw & Hmw & HF & #Hsm)".
@@ -496,16 +673,18 @@ Section UShPipesStage.
     iDestruct (shotsF_snoc with "Hsm HFs") as "#Hsn". rewrite -Hm.
     assert (Hwl : WLast ∈ wsN) by (apply wids_elem; done).
     assert (Hfd2 : UkSh.ush_fd2p ld) by (destruct Hfd as (_ & _ & Hf2); exact Hf2).
-    iAssert (pkitR WLast L) as "#HkL".
-    { rewrite /pns_kit. iSplit.
-      - iExists (EXf nc L WLast L). iSplitR.
-        + iPureIntro. exact (Hfire WLast L Hwl (or_introl eq_refl)).
-        + iApply (pexcl_last fc adm I L P gF gG L HLne HLne with "Hinvs").
-      - iPureIntro. intros c [Hc0 Hcl].
-        apply (cstep_okN_tok fc adm I Hadmit WLast L c Hc0 Hcl).
-        intros j Hj; discriminate Hj. }
-    iPoseProof (pdep_last_of_lb fc adm I L P gF gG HLne ltac:(lia) with "Hsn Hinvs")
-      as "#Hdw".
+    (* THE CONTENT WRITER'S KIT AND DEPOSIT, at a nonempty line *)
+    iAssert (⌜L = []⌝ ∨ (pkitR WLast L
+               ∗ □ (pws_lb (P (nc - 1)) (take 1 L) ={↑pipeN}=∗ pdepR WLast L)))%I as "#Hkd".
+    { destruct (decide (L = [])) as [HL0 | HLne]; [by iLeft |]. iRight. iSplit.
+      - rewrite /pns_kit. iSplit.
+        + iExists (EXf fc pr nc L WLast L). iSplitR.
+          * iPureIntro. exact (Hfire WLast L Hwl (or_introl (conj eq_refl HLne))).
+          * iApply (pexcl_last fc adm I L pr P gF gG L HLne with "Hinvs").
+        + iPureIntro. intros c [Hc0 Hcl].
+          apply (cstep_okN_tok fc adm I Hadmit WLast L c Hc0 Hcl).
+          intros j Hj; discriminate Hj.
+      - iApply (pdep_last_of_lb fc adm I L pr P gF gG HLne ltac:(lia) with "Hsn Hinvs"). }
     replace (nc - 1)%nat with m by lia.
     set (Cr := (rcur (P m) 0 ∗ side_R (P m)
                 ∗ wcurN γc WLast (1/2) 0 ∗ wmodeN γm WLast (1/2) None)%I).
@@ -528,11 +707,11 @@ Section UShPipesStage.
       + iIntros "!> (Hr & HsR & Hcw & Hmw)". rewrite /pns_copy_lend_m.
         iSplitR; [cbn [pns_pk_inv]; iSplit; [iExists (prevP P m); iExact "Hpo" | done] |].
         iFrame "Hr". iSplitL "Hcw Hmw".
-        { rewrite /pns_sink. iSplitR; [by iPureIntro |]. iFrame "Hinv HkL".
-          iSplitR; [iExact "Hdw" |]. cbn [pns_cmode]. iFrame "Hcw Hmw". }
+        { rewrite /pns_sink. iSplitR; [by iPureIntro |]. iSplitR; [iExact "Hinv" |].
+          iSplitR; [iExact "Hkd" |]. cbn [pns_cmode]. iFrame "Hcw Hmw". }
         rewrite /pns_xkQ. iIntros "[#HT | (_ & Hf1 & _)]"; [by iLeft |].
         cbn [pns_final snd].
-        iDestruct "Hf1" as (c) "(#Heof & _ & Hcw & Hmw)".
+        iDestruct "Hf1" as (c) "(%HcL & #Heof & _ & Hcw & Hmw)".
         iRight. iRight. iFrame "HsR". rewrite /rrep.
         iExists (RdEof (take c L)). replace (S m - 1)%nat with m by lia.
         cbn [rd_final]. iFrame "Heof". iLeft. rewrite /sufN.
@@ -547,7 +726,7 @@ Section UShPipesStage.
           rewrite /wlast. cbn [pns_cmode]. iFrame "Hcw Hmw".
           iPureIntro. lia.
       + iApply (pse_last_image_entry_m (PS := uprogSG_free) g fc adm LW Hcons Hkill rn Heq Hfc
-                  v I Hadmit Hplok L HL31 termw TOKN pdepR (pdep_timeless fc adm I L P gF gG)
+                  v I Hadmit Hplok L HL31 termw TOKN pdepR (pdep_timeless fc adm I L pr P gF gG)
                   γc γm a b M s1 t1 g1 sts FsImg.ROOTINO cs pidv (fun _ : Z => QcR m)
                   (P m) γp WLast wb rb1 rb2
                   (fun _ _ => eq_refl) Ht1 Hs1 Hb1 Hi1 Hl1 Hr0 Hr1 Hr2
@@ -555,7 +734,7 @@ Section UShPipesStage.
         iApply UexecExecMint.udep_free.
     - (* ---- THE EXEC-FAILED LAW: the content writer ---- *)
       iApply (exf_writer WLast dg_execR alt_execR 16%nat
-                (EXf nc L WLast dg_execR) Cr (side_R (P m)) Cd Hwl ltac:(lia)
+                (EXf fc pr nc L WLast dg_execR) Cr (side_R (P m)) Cd Hwl ltac:(lia)
                 ltac:(intros p b' Hp Hb; exact (dg_app_lookup dg_execR u_prompt p b'
                                ltac:(rewrite dg_execR_len; lia) Hb))
                 (Hfire WLast dg_execR Hwl (or_intror eq_refl))
@@ -563,9 +742,9 @@ Section UShPipesStage.
                       apply (cstep_okN_tok fc adm I Hadmit WLast dg_execR c);
                       [lia | rewrite dg_execR_len; lia | intros j Hj; discriminate Hj])
                 with "Hinv [] [] []").
-      + iApply (pexcl_last fc adm I L P gF gG dg_execR (dg_st_ne 1) HLne with "Hinvs").
+      + iApply (pexcl_last fc adm I L pr P gF gG dg_execR (dg_st_ne pr 1) with "Hinvs").
       + iIntros "!> (_ & HsR & Hcw & Hmw)". iFrame "HsR Hcw Hmw".
-        rewrite (pdep_unfold fc adm I L P gF gG WLast dg_execR (dg_st_ne 1)
+        rewrite (pdep_unfold fc adm I L pr P gF gG WLast dg_execR (dg_st_ne pr 1)
                    (or_intror eq_refl)) /pdep_ne.
         iFrame "Hsn". case_bool_decide as Hq; [| done]. iRight. by iPureIntro.
       + iIntros "!> HsR Hcw Hmw _". rewrite /Cd. iFrame "HsR".
